added filter facts, permutation invariant completely verified

DistinctElts.dfy
@@ -43,7 +43,7 @@ ensures(numLt_alt(x-1, a) == |filter (a, y => y < x - 1)|) {
 }
 
 function numLeq_alt(x: int, a : seq<int>) : int {
-  numLt_alt(x, a) + (if x in a then 1 else 0)
+  |filter(a, y => y <= x)|
 }
 
 /*lemma idx_exists<T>(a:seq<T>, x : T) 
@@ -110,9 +110,30 @@ requires(forall x : T :: x in a ==> ! f(x))
 ensures(filter(a, f) == []) {
 
 }
+
+lemma {: induction a} filter_eq_nodups(a:seq<int>, x : int)
+requires(noDups_seq(a))
+ensures(|filter(a, y => y == x)| == if (x in a) then 1 else 0) {
+}
+
+//for some reason Dafny cannot prove this from above
+lemma {: induction a} filter_eq_nodups_minus(a:seq<int>, x : int)
+requires(noDups_seq(a))
+ensures(|filter(a, y => y == x-1)| == if (x-1 in a) then 1 else 0) {
+}
+
+lemma {: induction a} filter_length_nodups(a: seq<int>, x : int)
+requires((x-1) in a)
+requires(noDups_seq(a))
+ensures(|filter(a, y => y == (x - 1))| == 1) {
+  filter_eq_nodups_minus(a, x);
+}
+
+
 //A key lemma - if a list contains no duplicates and an element x is in the list, keeping only the elements equal to x gives a singleton list
 //for some reason dafny doesn't like this with x, then plugging in x - 1 (maybe because of score of x in anonymous function) - so we use x-1 directly
-lemma {: induction a} filter_length_nodups(a: seq<int>, x: int)
+/*
+lemma {: induction a} filter_length_nodups'(a: seq<int>, x: int)
 requires((x- 1) in a)
 requires(noDups_seq(a))
 ensures(|filter(a, y => y == (x - 1))| == 1) {
@@ -131,6 +152,7 @@ ensures(|filter(a, y => y == (x - 1))| == 1) {
   filterEmpty(a[i+1..], y => y == (x - 1));
   assert(filter(a[i+1..], y => y == (x - 1)) == []);
 }
+*/
 
 /* the big one: linking the two implementations of numLt*/
 lemma {: induction x} numLt_equiv(x: int, a : seq<int>)
@@ -144,18 +166,11 @@ ensures(numLt(x, a) == numLt_alt(x,a)) {
     else {
       if((x-1) in a) {
         filter_lt_decompose(a, (x));
-        //assert((|filter(a, y => y < x)| == |filter(a, y => y < x - 1)| + |filter(a, y => y == x - 1)|));
         filter_length_nodups(a, x);
-        //assert(|filter(a, y => y == (x - 1))| == 1);
-        //assert(|filter(a, y => y < x)| == |filter(a, y => y < x - 1)| + 1);
         numLt_alt_minus(x, a);
-        //assert(numLt_alt(x-1, a) == |filter(a, y => y < x - 1)| );
-
-        //assert(numLt_alt(x, a) == 1 + numLt_alt(x-1, a));
       }
       else {
         filter_lt_decompose(a, (x));
-        //assert(forall y :: y in a ==> y != x);
         filterEmpty(a, y => y == (x - 1));
         numLt_alt_minus(x, a);
       }
@@ -167,6 +182,86 @@ ensures(numLt(x, a) == numLt_alt(x,a)) {
   2. filter definition - this is the meaning of the function (number of elts less than x) and makes it easy to prove bounds - 
      for instance, it is always <= length of list 
     We will also use this definition to prove transitivity and injectivity properties */
+
+//First, we define numLeq in terms of filter
+
+//dafny is magical
+lemma filter_leq_decompose(a: seq<int>, x : int)
+ensures(|filter(a, y => y <= x)| == |filter(a, y => y < x)| + |filter(a, y => y == x)|) {
+}
+
+lemma {: induction x} numLeq_equiv(x: int, a : seq<int>)
+requires(forall x : int :: x in a ==> x >= 0)
+requires(noDups_seq(a))
+ensures(numLeq(x, a) == numLeq_alt(x,a)) {
+  numLt_equiv(x, a);
+  filter_leq_decompose(a, x);
+  filter_eq_nodups(a, x);
+}
+
+/* Bounds on num_Leq - need for array checks */
+lemma {:induction x} numLt_nonneg(x: int, a : seq<int>)
+ensures(0 <= numLt(x,a)) {
+}
+
+lemma numLeq_nonneg(x: int, a : seq<int>)
+requires (x in a)
+ensures(1 <= numLeq(x,a)) {
+  numLt_nonneg(x, a);
+}
+
+lemma filter_length_leq<T>(a: seq<T>, f: T -> bool)
+ensures(|filter(a, f)| <= |a|) {
+
+}
+
+lemma numLeq_upper_bound(x: int, a : seq<int>)
+requires(forall x : int :: x in a ==> x >= 0)
+requires (noDups_seq(a))
+ensures(numLeq(x, a) <= |a|) {
+  numLeq_equiv(x, a);
+  filter_length_leq(a, y => y <= x);
+}
+
+//Now, we prove a form of injectivity for numLeq
+lemma {: induction a} filter_leq_decompose_bounds(a : seq<int>, x : int, y : int)
+requires (x < y)
+ensures (|filter(a, z => z <= y)| == |filter(a, z => z <= x)| + |filter(a, z => x < z && z <= y)|) {
+}
+
+lemma filter_bounded_in(a:seq<int>, x : int, y : int)
+requires(x < y)
+requires(y in a)
+ensures(|filter(a, z => x < z && z <= y)| > 0){
+}
+
+lemma numLeq_lt_trans(a:seq<int>, x: int, y: int)
+requires(x < y)
+requires(y in a)
+requires(forall x : int :: x in a ==> x >= 0)
+requires(noDups_seq(a))
+ensures(numLeq(x, a) < numLeq(y, a)) {
+  numLeq_equiv(x, a);
+  numLeq_equiv(y, a);
+  filter_leq_decompose_bounds(a, x, y);
+  filter_bounded_in(a, x, y);
+}
+
+lemma numLeq_inj(a:seq<int>, x : int, y : int)
+requires(x != y)
+requires(x in a)
+requires (y in a)
+requires(forall x : int :: x in a ==> x >= 0)
+requires(noDups_seq(a))
+ensures(numLeq(x, a) != numLeq(y, a)) {
+  if(x < y) {
+    numLeq_lt_trans(a, x, y);
+  }
+  else {
+    numLeq_lt_trans(a, y, x);
+  }
+}
+
 
 function seqSet<T>(a: seq<T>) : set<T> {
     set x : T | x in a
@@ -271,16 +366,16 @@ requires(0 < b.Length)
 requires(noDups(a))
 requires(forall i : int :: 0 <= i < b.Length ==> b[i] == (if i in a[..] then 1 else 0))
 ensures(c.Length == b.Length)
-ensures(forall i : int {:induction i} :: 0 <= i < b.Length ==> (c[i] == numLeq(i, a[..])));
+ensures(forall i : int {:induction i} :: 0 <= i < b.Length ==> (c[i] == numLeq(i, a[..]) - 1));
 {
   var i := 1;
   assert(numLeq(0, a[..]) == b[0]);
   c := new int[b.Length];
-  c[0] := b[0];
+  c[0] := b[0] - 1;
   while(i < c.Length)
   decreases (b.Length - i)
   invariant (1 <= i <= c.Length)
-  invariant(forall j: int {:induction j} :: (0 <= j < i ==> c[j] == numLeq(j, a[..])))
+  invariant(forall j: int {:induction j} :: (0 <= j < i ==> c[j] == numLeq(j, a[..]) - 1))
   //invariant(forall j: int :: i <= j < b.Length ==> b[j] == multiset(a[..])[j]) {
   {
     c[i] := b[i] + c[i-1];
@@ -288,11 +383,51 @@ ensures(forall i : int {:induction i} :: 0 <= i < b.Length ==> (c[i] == numLeq(i
   }
 }
 
+lemma prefixSumBounds(a: array<int>, b : array<int>, j : int)
+requires(forall i : int {:induction i} :: 0 <= i < b.Length ==> (b[i] == numLeq(i, a[..]) - 1))
+requires(forall i : int :: 0 <= i < a.Length ==> 0 <= a[i] < b.Length)
+requires(0 <= j < a.Length)
+requires(noDups(a))
+ensures(0 <= b[a[j]] < a.Length) {
+  assert(a[j] in a[..]);
+  numLeq_nonneg(a[j], a[..]);
+  numLeq_upper_bound(a[j], a[..]);
+}
+
+//puts this in a forall statement we can use - NOTE!!! this is how you introduce quanfitied vars in Dafny!
+lemma prefixSumBounds'(a: array<int>, b : array<int>)
+requires(forall i : int {:induction i} :: 0 <= i < b.Length ==> (b[i] == numLeq(i, a[..]) - 1))
+requires(forall i : int :: 0 <= i < a.Length ==> 0 <= a[i] < b.Length)
+requires(noDups(a))
+ensures(forall j : int {: induction j} :: 0 <= j < a.Length ==> 0 <= b[a[j]] < a.Length) {
+  //prefixSumBounds(a, b, j);
+  forall j : int | 0 <= j < a.Length {
+    prefixSumBounds(a, b, j);
+  }
+}
+
+//need this in loop to make sure we don't repeat
+lemma prefixSumInj(a: array<int>, b : array<int>, i: int)
+requires(noDups(a))
+requires(forall i : int {:induction i} :: 0 <= i < b.Length ==> (b[i] == numLeq(i, a[..]) - 1))
+requires(forall i : int :: 0 <= i < a.Length ==> 0 <= a[i] < b.Length)
+requires(0 <= i < a.Length)
+ensures(forall j : int :: 0 <= j <= i - 1 ==> b[a[j]] != b[a[i]]) {
+  forall j : int | 0 <= j <= i - 1
+   ensures (b[a[j]] != b[a[i]]) 
+   {
+    //NOTE: use noDups in non trivial way here - rely on fact that i != j -> a[i] != a[j]
+    numLeq_inj(a[..], a[i], a[j]);
+  }
+}
+
+
+
 //a is the original array, b is prefix sum array
 method constructSortedArray (a: array<int>, b: array<int>) returns (c : array<int>)
 requires(noDups(a))
 //requires(a.Length > 0)
-requires(forall i : int {:induction i} :: 0 <= i < b.Length ==> (b[i] == numLeq(i, a[..])));
+requires(forall i : int {:induction i} :: 0 <= i < b.Length ==> (b[i] == numLeq(i, a[..]) - 1));
 requires(forall i : int :: 0 <= i < a.Length ==> 0 <= a[i] < b.Length)
 
 //TODO: fill in postconditions
@@ -317,11 +452,13 @@ requires(forall i : int :: 0 <= i < a.Length ==> 0 <= a[i] < b.Length)
   filterEmpty(c[..], y => y >= 0);
   assert(filter(c[..], y => y >= 0) == []);
   assert(seqSet(a[(i+1)..a.Length]) == seqSet(filter(c[..], y => y >= 0)));
-  //assume((forall j: int :: 0 <= i < a.Length ==> 0 <= b[a[j]] < c.Length));\
-  assume(forall j: int :: 0 <= j < b.Length ==> 0 <= b[j] < c.Length); // TODO
+  //assume((forall j: int :: 0 <= i < a.Length ==> 0 <= b[a[j]] < c.Length));
+  prefixSumBounds'(a,b);
+  assert(forall j : int :: 0 <= j < a.Length ==> 0 <= b[a[j]] < a.Length); // TODO
   assert((forall j: int:: 0 <= j <= i ==> c[b[a[j]]] == -1));
 
   while(i >= 0)
+  decreases (i-0)
   invariant(-1 <= i < a.Length)
   invariant(forall j: int ::i < j < a.Length ==> 0 <= b[a[j]] < c.Length)
   invariant(forall j: int:: i < j < a.Length ==> c[b[a[j]]] >= 0)
@@ -332,7 +469,7 @@ requires(forall i : int :: 0 <= i < a.Length ==> 0 <= a[i] < b.Length)
 
     assert(0 <= i < a.Length);
     assert(0 <= a[i] < b.Length);
-    assume(0 <= b[a[i]] < c.Length);
+    assert(0 <= b[a[i]] < c.Length);
     //permutation invar
     assert(seqSet(a[i..a.Length]) == seqSet(a[(i+1)..a.Length]) + {a[i]} );
     assert(c[..] == (c[0..b[a[i]]] + [c[b[a[i]]]])+ c[b[a[i]] + 1..c.Length]);
@@ -353,7 +490,8 @@ requires(forall i : int :: 0 <= i < a.Length ==> 0 <= a[i] < b.Length)
     assert(a[i] != -1);
     assert(forall j: int:: 0 <= j <= i - 1 ==> c[b[a[j]]] == -1);
     //idea: noDups: i <> j -> a[i] <> a[j], so then by (injectivity), b[a[i]] <> b[a[j]]
-    assume(forall j : int :: 0 <= j <= i - 1 ==> b[a[j]] != b[a[i]]); // TODO; solve this goal
+    prefixSumInj(a, b, i);
+    //assume(forall j : int :: 0 <= j <= i - 1 ==> b[a[j]] != b[a[i]]); // TODO; solve this goal
     //assert(forall j : int :: 0 <= j <= i - 1 ==> c[b[a[j]]] == -1);
     c[b[a[i]]] := a[i];
     //also need to know that c[b[a[j]] <> c[b[a[i]]] - filtered part has nodups
